% arara: pdflatex
% arara: clean: { extensions: [ aux, blg, idx, ilg, ind, log, out, pytxcode, rel, toc ] }
% !arara: clean: { files: [ ans.tex, hint.tex] }

\documentclass[companion]{subfiles}

\begin{document}


\section{Renewal Reward Theorem}
\label{sec:renew-reward-theor}


We state the \recall{renewal reward theorem} and provide graphical motivation for its validity.
This result proves to be extremely useful: we will apply it regularly in the sequel of the book and here we use it to provide another definition of the load~$\rho$. 


\opt{solutionfiles}{
\subsection*{Theory and Exercises}
\Opensolutionfile{hint}
\Opensolutionfile{ans}
}


In essence the renewal reward theorem is very simple: it states that when customers arrive at rate $\lambda$ and each customer pays an average amount $X$, the system earns money at rate $Y=\lambda X$.
\Cref{fig:renewal} provides graphical motivation about why this theorem is true; \citet{el-taha98:_sampl_path_analy_queuein_system} gives a (simple) proof.

\begin{theorem}[Renewal Reward Theorem, $Y=\lambda X$]
 Consider epochs $\{T_k, k=0, 1, \ldots\}$ such that $0=T_0 < T_1 < \cdots$
 Let $N=\{N(t), t\geq 0\}$ be the associated counting process with $N(t) = \max\{k : T_k \leq t\}$.
 Let $\{Y(t), t\geq 0\}$ be a non-decreasing right-continuous (deterministic) process.
 Define $X_k = Y(T_k)-Y(T_{k-1})$.
 Suppose that $N(t)/t\to\lambda$ as $t\to\infty$, where $0<\lambda < \infty$.
 Then $Y(t)/t$ has a limit iff $n^{-1}\sum_{k=1}^n X_k$ has a limit, and then $Y=\lambda X$. In other words, 
 \begin{equation*}
 \lim_{t \to \infty} \frac{Y(t)}t=Y \iff \lim_{n \to \infty} \frac 1n\sum_{k=1}^n X_k = X, 
 \end{equation*}
and then $Y=\lambda X$. 
\end{theorem}


\begin{figure}[ht]
 \centering
\begin{tikzpicture}[scale=1]
%axis
\draw[->] (0,0) -- coordinate (x axis mid) (8.5,0);
\draw[->] (0,0) -- coordinate (y axis mid) (0,5.5);
%\node[below=0.2cm] at (x axis mid) {$t$};

\draw plot [smooth] coordinates {(1,0.7) (2,1) (3,1.8) (4,2) (5,3) (6,3.2) (7, 3.4) (7.5,4.0)};
\node[right] at (7.1,3.4) {$Y(t)$};
\node at (7.,-0.5) {$t$};

\node at (2.,-0.5) {$T_{k-1}$};
\draw[dotted] (2,0)--(2,1);
\draw[dotted] (2,1)--(3,1);


\node at (3.,-0.5) {$T_{k}$};
\draw[dotted] (3,0)--(3,1.8);
\draw[dotted] (3,1.8)--(5,1.8);

\draw [
 thick,
 decoration={brace, mirror, raise=0.1cm },
 decorate
] (3,1) -- (3,1.8)
node[pos=0.5, xshift=0.6cm] {$X_k$}; 


\node at (5.,-0.5) {$T_{k+1}$};
\draw[dotted] (5,0)--(5,3);

\draw [
 thick,
 decoration={brace, mirror, raise=0.1cm },
 decorate
] (5,1.8) -- (5,3)
node[pos=0.5, xshift=0.7cm] {$X_{k+1}$}; 

\node[right] at (0.5,4) {$\frac{Y(t)}t \approx \frac{\sum_i^n X_i}{T_n} = \frac{n}{T_n} \frac{\sum_i^n X_i}n $};


\draw[dotted,<->, =stealth] (7,0.05)--(7,3.35) node[midway, rotate=90, fill=white] {$\sum_{i=1}^n X_i$};
\draw[dotted,<->, =stealth] (0.05,0.5)--(6.95,0.5) node[pos=0.85, fill=white] {$T_n$};
\end{tikzpicture}
\caption{A graphical `proof' of $Y=\lambda X$. Here $Y(t)/t\to Y$, $n/T_n\to \lambda$ and $n^{-1}\sum_i^n X_i \to X$. Observe that in the
 figure $X_k$ does not represent an inter-arrival time; instead it
 corresponds to the increment of (the graph of) $Y(t)$ between two
 consecutive epochs $T_{k-1}$ and $T_k$ at which $Y(t)$ is
 observed.}
 \label{fig:renewal}
\end{figure}

Let us use this theorem to understand the idea of `load' in a different way. 
Define the \recall{load} or \recall{utilization} as the limiting fraction of time the server is busy, i.e.,
\begin{equation*}
 \rho = \lim_{t\to\infty} \frac 1 t \int_0^t \1{L(s)>0} \d s.
\end{equation*}

\begin{exercise}\clabel{ex:l-162}
Use the renewal reward theorem to prove that $\rho = \lambda \E S$ for the rate-stable $G/G/1$ queue. 
\begin{hint}
 Define $Y(t) = \int_0^t \1{L(s)>0} \d s$ as the total amount of time the server has been busy up to the time $t$.
 Then take as epochs $T_k = D_k$ and use rate stability.
\end{hint}
\begin{solution}
 It is evident that $X_k = Y(D_k)-Y(D_{k-1})=S_k$, hence $X = \lim_{n\to\infty} n^{-1}\sum_{k=1}^n X_k = \E S$.
 Also $\lim_{t\to\infty} Y(t)/t=\rho$.
 Finally, in the relation $Y = \lambda X$, the $\lambda$ is $\delta$ since we consider departure epochs $T_k = D_k$, rather than $A_k$.
 By the renewal reward theorem $Y=\lambda X$ we get that $\rho = \delta \E S$.
 Finally, by rate-stability, the job arrival rate $\lambda = \delta$, hence $\rho = \lambda \E S$.
\end{solution}
\end{exercise}


\begin{exercise}\clabel{ex:l-163}
 We can derive the relation $\rho = \lambda \E S$ in a somewhat more direct way by considering the fact that
\begin{equation*}
 \sum_{k=1}^{A(t)} S_k \geq \int_0^t \1{L(s)>0} \d s \geq \sum_{k=1}^{D(t)} S_k.
\end{equation*}
Explain this, and conclude that 
\begin{equation}\label{eq:86}
\lambda \E S \geq \rho \geq \delta \E S.
\end{equation}
Hence, if the system is rate-stable, $\delta=\lambda$, and then $\rho = \lambda \E S$. 
\begin{solution}
Observe that
since $t$ can lie half way a service interval and $A(t) \geq D(t)$. As
$A(t)\to \infty$ as $t\to\infty$,
\begin{equation*}
 \lim_{t\to\infty} \frac 1 t\sum_{k=1}^{A(t)} S_k = 
 \lim_{t\to\infty} \frac{A(t)}t \frac{1}{A(t)} \sum_{k=1}^{A(t)} S_k = 
 \lim_{t\to\infty} \frac{A(t)}t \cdot \lim_{t\to\infty}\frac{1}{A(t)} \sum_{k=1}^{A(t)} S_k = \lambda \E S.
\end{equation*}

Applying similar limits to the other inequality gives the 

Note that this is in fact the same argument as that underlies the renewal reward theorem. Henceforth we will just use the renewal reward theorem. 
\end{solution}
\end{exercise}



\opt{solutionfiles}{
\Closesolutionfile{hint}
\Closesolutionfile{ans}
\subsection*{Hints}
\input{hint}
\subsection*{Solutions}
\input{ans}
}

\end{document}


%%% Local Variables:
%%% mode: latex
%%% TeX-master: t
%%% End:
